got simproc working

Pullback/P/Basic.lean
@@ -10,7 +10,7 @@ class BasedType (α : Type) where
   valueType : α → Type
 
 /-- `Typed α A` means each element of α can be assigned a type in A -/
-class Typed (α A : Type) where
+class Typed (α : Type) (A : outParam Type) where
   type : α → A
 
 inductive PType (BaseType : Type) where
@@ -121,7 +121,7 @@ def RawPExpr.inferType {Const BaseType} [DecidableEq BaseType] [Typed Const (PTy
       body.inferType ((x, vT)::ctxRaw)
 | const c => some (Typed.type c)
 
-def RawPExpr.toPExpr {BaseType Const} [DecidableEq BaseType] [Typed Const (PType BaseType)] (ctxRaw : List (Name × PType BaseType)) :
+def RawPExpr.toPExpr {BaseType Const} [Typed Const (PType BaseType)] [DecidableEq BaseType] (ctxRaw : List (Name × PType BaseType)) :
   (e : RawPExpr Const BaseType) → (he : (e.inferType ctxRaw).isSome) →
     (PExpr Const BaseType (ctxRaw.map (·.2)) ((e.inferType ctxRaw).get he))
 | var x, he =>
@@ -177,198 +177,14 @@ def RawPExpr.toPExpr {BaseType Const} [DecidableEq BaseType] [Typed Const (PType
     PExpr.letE v' (body.toPExpr ((x, vT)::ctxRaw) hbody)
 | const c, he => .const c
 
-class HasType {Const BaseType} [DecidableEq BaseType] [Typed Const (PType BaseType)] (ctxRaw : List (Name × PType BaseType)) (e : RawPExpr (Const := Const) (BaseType := BaseType)) (ty : outParam (PType BaseType)) where
+class HasType {Const BaseType} [Typed Const (PType BaseType)] [DecidableEq BaseType] (ctxRaw : List (Name × PType BaseType)) (e : RawPExpr (Const := Const) (BaseType := BaseType)) (ty : outParam (PType BaseType)) where
   hasType : e.inferType ctxRaw = ty
 
 class HasVar {BaseType} (ctxRaw : List (Name × PType BaseType)) (name : Name) (ty : outParam (PType BaseType)) where
   hasVar : ctxRaw.find? (·.1 == name) = some (name, ty)
 
-def RawPExpr.toPExpr' {BaseType Const} [DecidableEq BaseType] [Typed Const (PType BaseType)] (ctxRaw : List (Name × PType BaseType)) (ty : PType BaseType) :
+def RawPExpr.toPExpr' {BaseType Const} [Typed Const (PType BaseType)] [DecidableEq BaseType]  (ctxRaw : List (Name × PType BaseType)) (ty : PType BaseType) :
   (e : RawPExpr Const BaseType) → [HasType ctxRaw e ty] →
     (PExpr Const BaseType (ctxRaw.map (·.2)) ty) :=
   fun e he =>
     cast (by grind [HasType]) (e.toPExpr ctxRaw (by grind [HasType]))
-
-namespace RawPExpr
-
-variable {BaseType Const} [DecidableEq BaseType] [Typed Const (PType BaseType)]
-
-
-instance instHasType_const (ctxRaw : List (Name × PType BaseType)) (c : Const) :
-  HasType ctxRaw (RawPExpr.const c : RawPExpr Const BaseType) (Typed.type c) :=
-  ⟨by simp [inferType]⟩
-
-instance instHasType_lam (ctxRaw : List (Name × PType BaseType)) (x : Name) (argT bodyT : PType BaseType)
-    (body : RawPExpr Const BaseType) [HasType ((x, argT)::ctxRaw) body bodyT] :
-  HasType ctxRaw (RawPExpr.lam x argT body : RawPExpr Const BaseType) (PType.fun argT bodyT) :=
-  ⟨by
-    have hbody : inferType ((x, argT) :: ctxRaw) body = some bodyT :=
-      HasType.hasType (ctxRaw := ((x, argT) :: ctxRaw)) (e := body) (ty := bodyT)
-    simp [inferType, hbody]
-  ⟩
-
-instance instHasType_letE (ctxRaw : List (Name × PType BaseType)) (x : Name)
-    (v body : RawPExpr Const BaseType) (vT bodyT : PType BaseType)
-    [HasType ctxRaw v vT] [HasType ((x, vT)::ctxRaw) body bodyT] :
-  HasType ctxRaw (RawPExpr.letE x v body : RawPExpr Const BaseType) bodyT :=
-  ⟨by
-    have hv : inferType ctxRaw v = some vT :=
-      HasType.hasType (ctxRaw := ctxRaw) (e := v) (ty := vT)
-    have hbody : inferType ((x, vT) :: ctxRaw) body = some bodyT :=
-      HasType.hasType (ctxRaw := ((x, vT) :: ctxRaw)) (e := body) (ty := bodyT)
-    simp [inferType, hv, hbody]
-  ⟩
-
-instance instHasType_app (ctxRaw : List (Name × PType BaseType)) (dom codom : PType BaseType) (f x : RawPExpr Const BaseType) [HasType ctxRaw f (PType.fun dom codom)] [HasType ctxRaw x dom] :
-  HasType ctxRaw (RawPExpr.app f x) codom :=
-  ⟨by simp [inferType]; grind [HasType]⟩
-
-instance instHasVar_head {ctx : List (Name × PType BaseType)} {name : Name} {ty : PType BaseType} :
-    HasVar ((name, ty) :: ctx) name ty :=
-  ⟨by grind⟩
-
-theorem hasVar_cons {ctx : List (Name × PType BaseType)} {name name' : Name} {ty ty' : PType BaseType}
-    {idx : Fin ctx.length}
-    (h : HasVar ctx name ty) (hne : name' ≠ name) :
-    HasVar ((name', ty') :: ctx) name ty :=
-  ⟨by grind [h.1]⟩
-
-instance instHasType_var {ctx : List (Name × PType BaseType)} {name : Name}
-  {ty : PType BaseType} [hv : HasVar ctx name ty] :
-    HasType ctx (RawPExpr.var name : RawPExpr Const BaseType) ty :=
-  ⟨by
-    {
-      have := hv.1
-      rw [List.find?_eq_some_iff_getElem] at this
-      simp [List.findFinIdx?_eq_some_iff, inferType, Option.bind_eq_some_iff]
-      obtain ⟨i, hi, H⟩ := this.2
-      use ⟨i, hi⟩
-      grind
-    }⟩
-
-macro "inferHasType" : tactic =>
-  `(tactic| (apply HasType.mk; simp [RawPExpr.inferType, List.findFinIdx?, List.findFinIdx?.go, Typed.type]))
-
-macro "inferHasVar" : tactic =>
-  `(tactic| (apply HasVar.mk; rfl))
-
-
-open Lean Meta Expr Elab Term Tactic Core IO LibrarySuggestions
-#check Simp.Context.ofArgs
-#check Lean.Meta.mkSimpTheoremFromExpr
-open Lean Meta Elab Tactic Simp in
-open Lean Meta
-/-- Simplify an expression using the given lemmas -/
-def simpExpr (e : Expr) (defns : List Name) : MetaM Expr := do
-  let cfg : Lean.Meta.Simp.Config := {
-    zeta := true
-    beta := true
-    eta := true
-    iota := true
-    proj := true
-    decide := false
-    contextual := false
-    arith := false
-  }
-  let ctx ← Meta.mkSimpContext (simpOnly := false) cfg
-
-  let mut simpTheorems := ctx.simpTheorems
-  if simpTheorems.isEmpty then
-    simpTheorems := #[]
-
-  -- 🔥 KEY CHANGE HERE
-  for name in defns do
-    simpTheorems ← simpTheorems.modifyM 0 fun thms0 =>
-      thms0.addDeclToUnfold name
-
-  let ctx := ctx.setSimpTheorems simpTheorems
-  let result ← Meta.simp e ctx
-  return result.1.expr
-
-open Lean Meta Elab Tactic Simp
-/-- Term elaborator that returns `RawPExpr.inferType vars e` unevaluated (no simplification). -/
-elab "exprTypeOf" e:term "in" vars:term : term => do
-  let stx ← `((RawPExpr.inferType $vars $e).get (by simp [RawPExpr.inferType, List.findFinIdx?, List.findFinIdx?.go, Typed.type]))
-  let e ← Lean.Elab.Term.elabTerm stx none
-  simpExpr e [`PExpr.RawPExpr.inferType, `List.findFinIdx?, `List.findFinIdx?.go, `Typed.type]
-
-end RawPExpr
-
-variable {Const Const' BaseType BaseType'} [DecidableEq BaseType] [BasedType BaseType] [BasedType BaseType'] [DecidableEq BaseType'] [Typed Const (PType BaseType)] [Typed Const' (PType BaseType')]
-variable [Interp BaseType Const] [Interp BaseType' Const']
-
-@[simp]
-theorem toPExpr'_app
-    {ctx : List (Name × PType BaseType)}
-    {f a : RawPExpr Const BaseType}
-    {A : PType BaseType}
-    {B : PType BaseType}
-    (hf : HasType ctx f (A.fun B) := by inferHasType) (ha : HasType ctx a A := by inferHasType) :
-  (RawPExpr.app f a).toPExpr' ctx B
-  =
-  PExpr.app
-    (f.toPExpr' ctx (A.fun B))
-    (a.toPExpr' ctx A) := by
-simp [RawPExpr.toPExpr', RawPExpr.toPExpr]
-rw! (castMode := .all) [hf.1]
-simp [ha.1]
-
-@[simp]
-theorem toPExpr'_const
-    {ctx : List (Name × PType BaseType)}
-    (c : Const) :
-  (RawPExpr.const c : RawPExpr Const BaseType).toPExpr' ctx (Typed.type c)
-  = PExpr.const c := by
-rfl
-
-@[simp]
-theorem toPExpr'_lam
-    {ctx : List (Name × PType BaseType)}
-    {x : Name} {argT bodyT : PType BaseType}
-    {body : RawPExpr Const BaseType}
-    (hbody : HasType ((x, argT) :: ctx) body bodyT := by inferHasType) :
-  (RawPExpr.lam x argT body : RawPExpr Const BaseType).toPExpr' ctx (.fun argT bodyT)
-  = PExpr.lam argT (body.toPExpr' ((x, argT) :: ctx) bodyT) := by
-simp [RawPExpr.toPExpr', RawPExpr.toPExpr]
-rw! (castMode := .all) [hbody.1]
-simp
-
-@[simp]
-theorem toPExpr'_letE
-    {ctx : List (Name × PType BaseType)}
-    {x : Name} {v body : RawPExpr Const BaseType}
-    {vT bodyT : PType BaseType}
-    (hv : HasType ctx v vT := by inferHasType) (hbody : HasType ((x, vT) :: ctx) body bodyT := by inferHasType) :
-  (RawPExpr.letE x v body : RawPExpr Const BaseType).toPExpr' ctx bodyT
-  = PExpr.letE (v.toPExpr' ctx vT) (body.toPExpr' ((x, vT) :: ctx) bodyT) := by
-simp [RawPExpr.toPExpr', RawPExpr.toPExpr]
-rw! (castMode := .all) [hv.1, hbody.1]
-grind
-
-@[simp]
-theorem toPExpr'_var
-    {ctx : List (Name × PType BaseType)}
-    {name : Name} {ty : PType BaseType}
-    (hv : HasVar ctx name ty := by inferHasVar) :
-  (RawPExpr.var name : RawPExpr Const BaseType).toPExpr' ctx ty
-  = PExpr.var (Fin.cast (by grind) ((ctx.findFinIdx? (·.1 == name)).get (by grind [HasVar]))) ty (by {
-    have := hv.1
-    sorry
-  }) := by
-  simp [RawPExpr.toPExpr', RawPExpr.toPExpr]
-  grind [HasVar]
-
-example
-  {ctx : List (Name × PType BaseType)} {ty : PType BaseType} (args : DVector (ctx.map (·.2.type)))
-  {e : RawPExpr Const BaseType} {e' : RawPExpr Const' BaseType'}
-  (f : PType BaseType → PType BaseType') (hf : ∀ ty : PType BaseType, ty.type = (f ty).type)
-  (he : HasType ctx e ty := by inferHasType) (he' : HasType (ctx.map (fun (x, v) => (x, f v))) e' (f ty) := by inferHasType)
-  (E : ty.type) (E' : (f ty).type)
-  (He : (e.toPExpr' ctx ty).interp (cast (by grind) args) = E)
-  (He' : (e'.toPExpr' (ctx.map (fun (x, t) => (x, f t))) (f ty)).interp (cast sorry args) = E')
-  (H : E ≍ E') :
-    let harg := by
-      apply congrArg
-      simp
-      grind
-    (e.toPExpr ctx (by grind [HasType])).interp (cast (by grind) args) = cast (by simp [he.1, he'.1, hf]) ((e'.toPExpr (ctx.map (fun (x, t) => (x, f t))) (by grind [HasType])).interp (cast harg args)) := sorry
